Cleaned up ALU related theorems

Scratch.thy
@@ -24,14 +24,7 @@ lemma NAND_0_b [simp]: "NAND 0 b = 1"
   by (case_tac b) auto
 
 theorem NAND_comm: "NAND a b = NAND b a"
-proof (cases b)
-  assume "b = 0"
-  thus ?thesis using NAND_a_0 NAND_0_b by auto
-next
-  assume A1: "b = 1"
-  have "NAND a 1 = NAND 1 a" by (case_tac a) auto
-  thus ?thesis using A1 by simp
-qed
+  by (case_tac b; case_tac a) auto
 
 definition NOT :: \<open>bit \<Rightarrow> bit\<close>
   where [simp]: \<open>NOT a \<equiv> (NAND a a)\<close>
@@ -73,23 +66,11 @@ lemma AND_0_b [simp]: "AND 0 b = 0"
   by (case_tac b) auto
 
 theorem AND_comm: "AND a b = AND b a"
-proof (cases b)
-  case zero
-  thus ?thesis using AND_0_b AND_a_0 by simp
-next
-  case one
-  thus ?thesis using AND_1_b AND_a_1 by simp
-qed
+  using AND_0_b AND_a_0 AND_1_b AND_a_1 by (case_tac b) auto
 
 \<comment>\<open>We can prove that NAND really is just "NOT AND"!\<close>
 lemma NOT_AND_is_NAND: "NOT (AND a b) = NAND a b"
-proof (cases a)
-  case zero
-  thus ?thesis by simp
-next
-  case one
-  thus ?thesis by (case_tac b) auto
-qed
+  by (case_tac b; case_tac a) auto
 
 definition OR :: \<open>bit \<Rightarrow> bit \<Rightarrow> bit\<close>
   where [simp]: \<open>OR a b \<equiv> NAND (NOT a) (NOT b)\<close>
@@ -173,14 +154,11 @@ lemma DMUX_right [simp]: "DMUX i 1 = (0, i)"
   using AND_a_1 DMUX_def by auto
 
 (* Only 9 NAND gates are needed for the FULLADDER, returns (sum, carry). *)
-definition FULLADDER :: \<open>bit \<Rightarrow> bit \<Rightarrow> bit \<Rightarrow> (bit * bit)\<close>
-  where \<open>FULLADDER a b c \<equiv> let nab = NAND a b 
-in let sab = NAND (NAND b nab) (NAND a nab)
-in let scab = NAND sab c
-in (NAND (NAND scab sab) (NAND scab c), NAND nab scab)\<close>
-
-value "FULLADDER a b c"
-value "FULLADDER 1 0 1"
+definition FULLADDER :: \<open>bit \<Rightarrow> bit \<Rightarrow> bit \<Rightarrow> (bit * bit)\<close> where
+  "FULLADDER a b c \<equiv> let nab = NAND a b 
+  in let sab = NAND (NAND b nab) (NAND a nab)
+  in let scab = NAND sab c
+  in (NAND (NAND scab sab) (NAND scab c), NAND nab scab)"
 
 lemma FULLADDER_000 [simp]: "FULLADDER 0 0 0 = (0, 0)"
   by (simp add: FULLADDER_def)
@@ -220,7 +198,14 @@ proof -
 qed
 
 lemma FULLADDER_a0c: "FULLADDER a 0 c = (XOR a c,AND a c)"
-  by (smt (z3) FULLADDER_010 FULLADDER_011 FULLADDER_0bc FULLADDER_100 FULLADDER_101 bit_not_one_iff)
+proof - (* 18 ms *)
+  have f1: "FULLADDER 1 0 0 = (1, 0)"
+    using FULLADDER_100 by blast
+  have "FULLADDER 0 1 0 = (1, 0)"
+    using FULLADDER_010 by blast
+  then show ?thesis
+    using f1 by (smt (z3) FULLADDER_011 FULLADDER_0bc FULLADDER_101 bit_not_zero_iff)
+qed
 
 lemma FULLADDER_a00: "FULLADDER a 0 0 = (a,0)"
   by (case_tac a) auto
@@ -229,13 +214,33 @@ lemma FULLADDER_0b0: "FULLADDER 0 b 0 = (b,0)"
   by (case_tac b) auto
 
 lemma FULLADDER_abc: "FULLADDER a b c = (XOR a (XOR b c),OR (AND a b) (AND c (XOR a b)))"
-  by (smt (z3) AND_0_0 AND_1_0 AND_a_1 FULLADDER_000 FULLADDER_001 FULLADDER_010 FULLADDER_011 FULLADDER_100 FULLADDER_101 FULLADDER_110 FULLADDER_111 OR_0_b OR_1_0 XOR_0_0 XOR_0_1 XOR_1_0 XOR_1_1 bit_not_one_iff)
+proof - (* 72ms *)
+  { assume "0 \<noteq> b"
+    moreover
+    { assume "0 \<noteq> b \<and> 0 \<noteq> a"
+      then have "0 \<noteq> c \<and> 0 \<noteq> b \<and> 0 \<noteq> a \<or> FULLADDER 1 1 c = (XOR 1 (XOR 1 c), 1) \<and> 0 \<noteq> a \<and> 0 \<noteq> b"
+        using FULLADDER_110 XOR_1_0 XOR_1_1 by presburger
+      then have ?thesis
+        by fastforce }
+    ultimately have "1 = a \<longrightarrow> FULLADDER a b c = (XOR a (XOR b c), OR (AND a b) (AND c (XOR a b)))"
+      by blast }
+  moreover
+  { assume "1 \<noteq> a"
+    then have "1 \<noteq> a \<and> 1 \<noteq> b \<or> (XOR 0 (XOR b 0), 0::bit) = (b, 0) \<and> 1 \<noteq> c \<and> 1 \<noteq> a \<or> FULLADDER 0 b c = (XOR 0 (XOR b c), AND c (XOR 0 b)) \<and> 1 \<noteq> a"
+      using AND_1_b FULLADDER_011 XOR_0_0 XOR_0_1 XOR_1_0 XOR_1_1 by presburger
+    then have "(XOR 0 (XOR b 0), 0::bit) = (b, 0) \<and> 1 \<noteq> c \<and> 1 \<noteq> a \<or> FULLADDER 0 b c = (XOR 0 (XOR b c), AND c (XOR 0 b)) \<and> 1 \<noteq> a"
+      by fastforce
+    then have ?thesis
+      using FULLADDER_0b0 OR_0_b by fastforce }
+  ultimately show ?thesis
+    by (smt (z3) AND_0_b AND_1_b FULLADDER_101 FULLADDER_a00 OR_0_b XOR_0_0 XOR_0_1 XOR_1_0 XOR_1_1 bit_not_zero_iff)
+qed
 
 lemma FULLADDER_carry_criteria: "(s,1) = FULLADDER a b c \<longrightarrow> (a = 1 \<and> b = 1) \<or> (c = 1 \<and> a = 1 \<and> b = 0) \<or> (c = 1 \<and> a = 0 \<and> b = 1)"
 proof - (* 55ms, fastest proof I could find *)
-  have f1: "1 = c \<or> c = 0"
+  have A1: "1 = c \<or> c = 0"
     by force
-  have f2: "1 = b \<or> b = 0"
+  have A2: "1 = b \<or> b = 0"
     by force
   have "1 = a \<or> a = 0"
     by force
@@ -244,11 +249,11 @@ proof - (* 55ms, fastest proof I could find *)
     then have "1 = a \<longrightarrow> (s, 1) \<noteq> FULLADDER a b c \<or> 1 = a \<and> 1 = b \<or> 1 = c \<and> 1 = a \<and> b = 0 \<or> 1 = c \<and> a = 0 \<and> 1 = b"
       by simp }
   ultimately show ?thesis
-    using f2 f1 by (smt (z3) FULLADDER_000 FULLADDER_001 FULLADDER_010 FULLADDER_100 Pair_inject)
+    using A2 A1 by (smt (z3) FULLADDER_000 FULLADDER_001 FULLADDER_010 FULLADDER_100 Pair_inject)
 qed
 
 theorem FULLADDER_comm: "FULLADDER a b c = FULLADDER b a c"
-proof -
+proof - (* 82 ms *)
   have "\<forall>b. (b::bit) = 1 \<or> b = 0"
     using bit_not_zero_iff by blast
   then show ?thesis
@@ -352,12 +357,10 @@ fun bit_to_nat :: "bit \<Rightarrow> nat" where
 | "bit_to_nat 1 = 1"
 
 lemma bit_unsigned_max: "bit_to_nat b < 2"
-  apply (case_tac b; simp)
-  done
+  by (case_tac b) auto
 
 lemma bit_to_nat_ubound: "bit_to_nat b \<le> 1"
-  apply (case_tac b; simp)
-  done
+  by (case_tac b) auto
 
 fun Hex_to_nat :: "Hex \<Rightarrow> nat" where
   "Hex_to_nat (Hex a b c d) = (bit_to_nat d) + 2*(bit_to_nat c)
@@ -420,8 +423,7 @@ lemma Hex_to_nat_mod16 [simp]: "(Hex_to_nat x) mod 16 = Hex_to_nat x"
 (* I hate tactical proofs, but if I wrote this out in structured Isar, it'd be ridiculously long
 and boil down to "by simp" repeated over and over. *)
 theorem Hex_to_nat_to_Hex: "nat_to_Hex (Hex_to_nat a) = a"
-  apply (case_tac a; case_tac x1; case_tac x2; case_tac x3; case_tac x4; simp)
-  done
+  by (case_tac a; case_tac x1; case_tac x2; case_tac x3; case_tac x4) simp+
 
 fun nat_to_Word :: "nat \<Rightarrow> Word" where
 "nat_to_Word n = Word (nat_to_Hex ((n div 4096) mod 16)) (nat_to_Hex ((n div 256) mod 16))
@@ -446,8 +448,8 @@ qed
 lemma Word_to_nat_mod65536: "(Word_to_nat w) mod 65536 = Word_to_nat w"
   by (simp add: Word_unsigned_max)
 
-fun sign_bit :: "Word \<Rightarrow> bit" where
-"sign_bit (Word (Hex s _ _ _) _ _ _) = s"
+fun sign_bit :: \<open>Word \<Rightarrow> bit\<close> where
+  "sign_bit (Word (Hex s _ _ _) _ _ _) = s"
 
 section \<open>Logic Gates for Hexadecimals\<close>
 
@@ -455,31 +457,21 @@ fun NOT_Hex :: \<open>Hex \<Rightarrow> Hex\<close>
   where \<open>NOT_Hex (Hex a b c d) = Hex (NOT a) (NOT b) (NOT c) (NOT d)\<close>
 
 lemma NOT_NOT_Hex: "NOT_Hex (NOT_Hex a) = a"
-proof (cases a)
-  case (Hex x1 x2 x3 x4)
-  then show ?thesis using NOT_NOT by auto
-qed
+  using NOT_NOT by (case_tac a) auto
 
 fun AND_Hex :: \<open>Hex \<Rightarrow> Hex \<Rightarrow> Hex\<close> where
   "AND_Hex (Hex a1 b1 c1 d1) (Hex a2 b2 c2 d2) = Hex (AND a1 a2) (AND b1 b2) (AND c1 c2) (AND d1 d2)"
 
 lemma AND_Hex_x_F: "AND_Hex x XF = x"
-proof (cases x)
-  case (Hex x1 x2 x3 x4)
-  then show ?thesis using AND_a_1 by simp
-qed
+  using AND_a_1 by (case_tac x) simp
 
 lemma AND_Hex_F_x: "AND_Hex XF x = x"
-proof (cases x)
-  case (Hex x1 x2 x3 x4)
-  then show ?thesis using AND_1_b by simp
-qed
+  using AND_1_b by (case_tac x) simp
 
 fun OR_Hex :: \<open>Hex \<Rightarrow> Hex \<Rightarrow> Hex\<close> where
   "OR_Hex (Hex a1 b1 c1 d1) (Hex a2 b2 c2 d2) = Hex (OR a1 a2) (OR b1 b2) (OR c1 c2) (OR d1 d2)"
 
 lemma NOT_AND_NOT_Hex: "NOT_Hex (AND_Hex (NOT_Hex a) (NOT_Hex b)) = OR_Hex a b"
- 
 proof (cases a)
   case A: (Hex a1 a2 a3 a4)
   then show ?thesis
@@ -493,15 +485,15 @@ fun XOR_Hex :: \<open>Hex \<Rightarrow> Hex \<Rightarrow> Hex\<close> where
   "XOR_Hex (Hex a1 b1 c1 d1) (Hex a2 b2 c2 d2) = Hex (XOR a1 a2) (XOR b1 b2) (XOR c1 c2) (XOR d1 d2)"
 
 definition MUX_Hex :: \<open>Hex \<Rightarrow> Hex \<Rightarrow> bit \<Rightarrow> Hex\<close> where [simp]:
-  "MUX_Hex a b s \<equiv> case a of (Hex a1 b1 c1 d1) \<Rightarrow> (case b of (Hex a2 b2 c2 d2) \<Rightarrow> Hex (MUX a1 a2 s) (MUX b1 b2 s) (MUX c1 c2 s) (MUX d1 d2 s))"
+  "MUX_Hex a b s \<equiv> case a of (Hex a1 b1 c1 d1)
+                   \<Rightarrow> (case b of (Hex a2 b2 c2 d2)
+                     \<Rightarrow> Hex (MUX a1 a2 s) (MUX b1 b2 s) (MUX c1 c2 s) (MUX d1 d2 s))"
 
 lemma MUX_Hex_left [simp]: "MUX_Hex a b 0 = a"
-  apply (case_tac a; case_tac b; simp)
-  done
+  by (case_tac a; case_tac b) simp
 
 lemma MUX_Hex_right [simp]: "MUX_Hex a b 1 = b"
-  apply (case_tac a; case_tac b; simp)
-  done
+  by (case_tac a; case_tac b) simp
 
 section \<open>Logic Gates for Words\<close>
 
@@ -511,101 +503,68 @@ fun OR8 :: \<open>Hex \<Rightarrow> Hex \<Rightarrow> bit\<close> where
 lemma OR8_zero: "OR8 (0 :: Hex) (0 :: Hex) = 0"
   by (simp add: zero_Hex_def)
 
-lemma OR8_zero_iff_zero: "OR a b = 0 \<longleftrightarrow> a = 0 \<and> b = 0"
+lemma OR_zero_iff_zero: "OR a b = 0 \<longleftrightarrow> a = 0 \<and> b = 0"
   using NAND.elims by fastforce
+
+lemma OR8_zero_implies_zero: "OR8 a b = 0 \<longrightarrow> a = 0 \<and> b = 0"
+  by (smt (z3) Hex.exhaust OR8.simps OR_zero_iff_zero zero_Hex_def)
+
+lemma OR8_zero_if_zero: "a = 0 \<and> b = 0 \<longrightarrow> OR8 a b = 0"
+  by (simp add: zero_Hex_def)
+
+lemma OR8_zero_iff_zero: "OR8 a b = 0 \<longleftrightarrow> a = 0 \<and> b = 0"
+  using OR8_zero_implies_zero OR8_zero_if_zero by blast
 
 fun ISZERO16 :: \<open>Word \<Rightarrow> bit\<close> where
   "ISZERO16 (Word a b c d) = NOT (OR (OR8 a b) (OR8 c d))"
 
 lemma ISZERO16_check: "ISZERO16 (Word 0 0 0 0) = 1" by (simp add: OR8_zero)
 
+lemma ISZERO16_implies_zero: "ISZERO16 (Word a b c d) = 1 \<longrightarrow> a = 0 \<and> b = 0 \<and> c = 0 \<and> d = 0"
+  by (metis (full_types) ISZERO16.simps NOT_1 OR8_zero_iff_zero OR_1_0 OR_a_1 bit_not_one_iff) (* 111 ms *)
+
 lemma ISZERO16_zero: "ISZERO16 (Word a b c d) = 1 \<longleftrightarrow> a = 0 \<and> b = 0 \<and> c = 0 \<and> d = 0"
-proof
-  assume A1: "ISZERO16 (Word a b c d) = 1"
-  then have "NOT (OR (OR8 a b) (OR8 c d)) = 1" by simp
-  then have "OR (OR8 a b) (OR8 c d) = 0" using NAND.elims by auto
-  then have A2: "(OR8 a b) = 0 \<and> (OR8 c d) = 0" by (metis OR_0_b OR_1_b bit_not_zero_iff)
-  then show "a = 0 \<and> b = 0 \<and> c = 0 \<and> d = 0"
-    by (metis (no_types, lifting) Hex.exhaust OR8.simps OR8_zero_iff_zero zero_Hex_def)
-next
-  assume A1: "a = 0 \<and> b = 0 \<and> c = 0 \<and> d = 0"
-  then have "OR8 a b = 0 \<and> OR8 c d = 0" by (simp add: OR8_zero)
-  then have "OR (OR8 a b) (OR8 c d) = 0" by simp
-  then have "NOT (OR (OR8 a b) (OR8 c d)) = 1" by simp
-  then show "ISZERO16 (Word a b c d) = 1" using A1 by auto
-qed
+  using ISZERO16_check ISZERO16_implies_zero by blast
 
 fun NOT16 :: \<open>Word \<Rightarrow> Word\<close> where
   "NOT16 (Word a b c d) = Word (NOT_Hex a) (NOT_Hex b) (NOT_Hex c) (NOT_Hex d)"
+
+lemma NOT16_zero: "NOT16 (Word 0 0 0 0) = Word XF XF XF XF"
+  by (simp add: zero_Hex_def)
 
 lemma NOT16_one: "NOT16 (Word 0 0 0 1) = (Word XF XF XF XE)"
   by (simp add: one_Hex_def zero_Hex_def)
 
 lemma NOT16_NOT16: "NOT16 (NOT16 w) = w"
-proof (cases w)
-  case (Word w1 w2 w3 w4)
-  then show ?thesis using NOT_NOT_Hex by auto
-qed
+  using NOT_NOT_Hex by (case_tac w) auto
 
 fun AND16 :: \<open>Word \<Rightarrow> Word \<Rightarrow> Word\<close> where
   "AND16 (Word a1 a2 a3 a4) (Word b1 b2 b3 b4) = Word (AND_Hex a1 b1) (AND_Hex a2 b2) (AND_Hex a3 b3) (AND_Hex a4 b4)"
 
 lemma AND16_x_FFFF: "AND16 x (Word XF XF XF XF) = x"
-proof (cases x)
-  case (Word x1 x2 x3 x4)
-  then show ?thesis using AND_Hex_x_F by auto
-qed
+  using AND_Hex_x_F by (case_tac x) auto
 
 lemma AND16_FFFF_x: "AND16 (Word XF XF XF XF) x = x"
-proof (cases x)
-  case (Word x1 x2 x3 x4)
-  then show ?thesis using AND_Hex_F_x by auto
-qed
+  using AND_Hex_F_x by (case_tac x) auto
 
 fun OR16 :: \<open>Word \<Rightarrow> Word \<Rightarrow> Word\<close> where
   "OR16 (Word a1 a2 a3 a4) (Word b1 b2 b3 b4) = Word (OR_Hex a1 b1) (OR_Hex a2 b2) (OR_Hex a3 b3) (OR_Hex a4 b4)"
 
 lemma NOT16_AND16_NOT16: "NOT16 (AND16 (NOT16 a) (NOT16 b)) = OR16 a b"
-proof (cases a)
-  case A: (Word a1 a2 a3 a4)
-  then show ?thesis
-  proof (cases b)
-    case (Word b1 b2 b3 b4)
-    then show ?thesis by (simp add: A NOT_AND_NOT_Hex)
-  qed
-qed
+  by (case_tac a; case_tac b) (simp add: NOT_AND_NOT_Hex)
 
 fun MUX16 :: \<open>Word \<Rightarrow> Word \<Rightarrow> bit \<Rightarrow> Word\<close> where
   "MUX16 (Word a1 b1 c1 d1) (Word a2 b2 c2 d2) s = Word (MUX_Hex a1 a2 s) (MUX_Hex b1 b2 s) (MUX_Hex c1 c2 s) (MUX_Hex d1 d2 s)"
 
 lemma MUX16_left [simp]: "MUX16 a b 0 = a"
-proof (cases a)
-  case A1: (Word a1 a2 a3 a4)
-  then show ?thesis
-  proof (cases b)
-    case A2: (Word y1 y2 y3 y4)
-    then show ?thesis using A1 MUX_Hex_left by auto
-  qed
-qed
+  using MUX_Hex_left by (case_tac a; case_tac b) simp
 
 lemma MUX16_right [simp]: "MUX16 a b 1 = b"
-proof (cases a)
-  case A1: (Word a1 a2 a3 a4)
-  then show ?thesis
-  proof (cases b)
-    case A2: (Word y1 y2 y3 y4)
-    then show ?thesis using A1 MUX_Hex_right by auto
-  qed
-qed
+  using MUX_Hex_right by (case_tac a; case_tac b) simp
 
 section \<open>Arithmetic Gates for Hex and Words\<close>
+
 (* Chained FULLADDERs returning the sum and its carry bit. *)
-(* fun ADDER_Hex :: \<open>Hex \<Rightarrow> Hex \<Rightarrow> bit \<Rightarrow> Hex * bit\<close> where
-"ADDER_Hex (Hex a1 a2 a3 a4) (Hex b1 b2 b3 b4) c = (let (s4,c4) = FULLADDER a4 b4 c
-in let (s3,c3) = FULLADDER a3 b3 c4
-in let (s2,c2) = FULLADDER a2 b2 c3
-in let (s1,c1) = FULLADDER a1 b1 c2
-in (Hex s1 s2 s3 s4, c1))" *)
 definition ADDER_Hex :: \<open>Hex \<Rightarrow> Hex \<Rightarrow> bit \<Rightarrow> Hex * bit\<close> where
 "ADDER_Hex a b c \<equiv> (case a of (Hex a1 a2 a3 a4) \<Rightarrow> case b of (Hex b1 b2 b3 b4) \<Rightarrow>
  (Hex (fst (FULLADDER a1 b1 (snd (FULLADDER a2 b2 (snd (FULLADDER a3 b3 (snd (FULLADDER a4 b4 c)))))))) (fst (FULLADDER a2 b2 (snd (FULLADDER a3 b3 (snd (FULLADDER a4 b4 c)))))) (fst (FULLADDER a3 b3 (snd (FULLADDER a4 b4 c)))) (fst (FULLADDER a4 b4 c)), (snd (FULLADDER a1 b1 (snd (FULLADDER a2 b2 (snd (FULLADDER a3 b3 (snd (FULLADDER a4 b4 c))))))))))"
@@ -634,99 +593,70 @@ lemma ADDER_Hex_alias: "(s4,c4) = FULLADDER a4 b4 c \<and> (s3,c3) = FULLADDER a
   by (smt (verit, ccfv_threshold) ADDER_Hex_simps prod.simps(2))
 
 lemma ADDER_Hex_0b0: "ADDER_Hex (Hex 0 0 0 0) b 0 = (b, 0)"
-proof (cases b)
-  case A1: (Hex b1 b2 b3 b4)
-  then show ?thesis using A1 FULLADDER_0b0 by auto
-qed
+  using FULLADDER_0b0 by (case_tac b) auto
 
 lemma ADDER_Hex_a00: "ADDER_Hex a (Hex 0 0 0 0) 0 = (a, 0)"
-proof (cases a)
-  case A1: (Hex a1 a2 a3 a4)
-  then show ?thesis using A1 FULLADDER_a00 by auto
-qed
+  using FULLADDER_a00 by (case_tac a) auto
 
-(* Again, I hate this, but grinding through each case is faster than an unenlightening
- Isar proof *)
-lemma ADDER_Hex_check: "Hex_to_nat (fst (ADDER_Hex a b 0)) = ((Hex_to_nat a) + (Hex_to_nat b)) mod 16"
-  apply (case_tac a; case_tac x1; case_tac x2; case_tac x3; case_tac x4)
-  apply (case_tac b; case_tac x1a; case_tac x2a; case_tac x3a; case_tac x4a; auto)+
+(* Brute force check all situations. It's not clever, but the readable Isar proof is too long
+   and about as interesting as Homer's catalogue of ships.
+
+   Although this suffices for now, it seems that there's some logic which could be refactored
+   out of ADDER16_check's proof to improve the proof-time for this theorem. *)
+theorem ADDER_Hex_check_carry: "(s, c :: bit) = ADDER_Hex a b c2 \<longrightarrow>
+  (Hex_to_nat a) + (Hex_to_nat b) + (bit_to_nat c2) = 16*(bit_to_nat c) + (Hex_to_nat s)"
+  apply (case_tac a; case_tac c; case_tac c2; case_tac x1; case_tac x2; case_tac x3; case_tac x4)
+  apply (simp add: ADDER_Hex_0b0)
+  apply (case_tac b; case_tac x1a; case_tac x2a; case_tac x3a; case_tac x4a; simp)+
   done
 
-lemma ADDER_Hex_small: "(Hex_to_nat a) + (Hex_to_nat b) < 16 \<longrightarrow> (s,0 :: bit) = ADDER_Hex a b 0 \<longrightarrow> (Hex_to_nat a) + (Hex_to_nat b) = (Hex_to_nat s)"
-proof -
-  have "s = fst (s, 0::bit)"
-    by auto
+corollary ADDER_Hex_check4: "(s,c) = ADDER_Hex a b 0 \<longrightarrow> (Hex_to_nat a) + (Hex_to_nat b) = 16*(bit_to_nat c) + (Hex_to_nat s)"
+  using ADDER_Hex_check_carry by fastforce
+
+corollary ADDER_Hex_check2: "(s,0 :: bit) = ADDER_Hex a b 0 \<longrightarrow> (Hex_to_nat a) + (Hex_to_nat b) = (Hex_to_nat s)"
+  using ADDER_Hex_check_carry by fastforce
+
+corollary ADDER_Hex_check3: "(s,1 :: bit) = ADDER_Hex a b 0 \<longrightarrow> (Hex_to_nat a) + (Hex_to_nat b) = 16 + (Hex_to_nat s)"
+  using ADDER_Hex_check_carry by fastforce
+
+corollary ADDER_Hex_check_carry2: "(s,0 :: bit) = ADDER_Hex a b 1 \<longrightarrow> (Hex_to_nat a) + (Hex_to_nat b) + 1 = (Hex_to_nat s)"
+  using ADDER_Hex_check_carry by fastforce
+
+corollary ADDER_Hex_check_carry3: "(s,1 :: bit) = ADDER_Hex a b 1 \<longrightarrow> (Hex_to_nat a) + (Hex_to_nat b) + 1 = 16 + (Hex_to_nat s)"
+  using ADDER_Hex_check_carry by fastforce
+
+corollary ADDER_Hex_check: "Hex_to_nat (fst (ADDER_Hex a b 0)) = ((Hex_to_nat a) + (Hex_to_nat b)) mod 16"
+proof - (* 5 ms *)
+  have "Hex_to_nat a + Hex_to_nat b = 16 * bit_to_nat (snd (ADDER_Hex a b 0)) + Hex_to_nat (fst (ADDER_Hex a b 0))"
+    by (simp add: ADDER_Hex_check4)
   then show ?thesis
-    by (smt (z3) ADDER_Hex_check mod_less)
+    by simp
 qed
 
-lemma ADDER_Hex_check2: "(s,0 :: bit) = ADDER_Hex a b 0 \<longrightarrow> (Hex_to_nat a) + (Hex_to_nat b) = (Hex_to_nat s)"
-  apply (case_tac a; case_tac x1; case_tac x2; case_tac x3; case_tac x4)
-  apply (case_tac b; case_tac x1a; case_tac x2a; case_tac x3a; case_tac x4a; auto)+
-  done
-
-lemma ADDER_Hex_check3: "(s,1 :: bit) = ADDER_Hex a b 0 \<longrightarrow> (Hex_to_nat a) + (Hex_to_nat b) = 16 + (Hex_to_nat s)"
-  apply (case_tac a; case_tac x1; case_tac x2; case_tac x3; case_tac x4)
-  apply (case_tac b; case_tac x1a; case_tac x2a; case_tac x3a; case_tac x4a; simp)+
-  done
-
-theorem ADDER_Hex_checks: "(s,c :: bit) = ADDER_Hex a b 0 \<longrightarrow>
-  (Hex_to_nat a) + (Hex_to_nat b) = (if (c=1) then 16 else 0) + (Hex_to_nat s)"
-  by (simp add: ADDER_Hex_check2 ADDER_Hex_check3)
-
-lemma ADDER_Hex_check_carry2: "(s,0 :: bit) = ADDER_Hex a b 1 \<longrightarrow> (Hex_to_nat a) + (Hex_to_nat b) + 1 = (Hex_to_nat s)"
-  apply (case_tac a; case_tac x1; case_tac x2; case_tac x3; case_tac x4)
-  apply (case_tac b; case_tac x1a; case_tac x2a; case_tac x3a; case_tac x4a; simp)+
-  done
-
-lemma ADDER_Hex_check_carry3: "(s,1 :: bit) = ADDER_Hex a b 1 \<longrightarrow> (Hex_to_nat a) + (Hex_to_nat b) + 1 = 16 + (Hex_to_nat s)"
-  apply (case_tac a; case_tac x1; case_tac x2; case_tac x3; case_tac x4)
-  apply (case_tac b; case_tac x1a; case_tac x2a; case_tac x3a; case_tac x4a; fastforce)+
-  done
-
-theorem ADDER_Hex_check_carry: "(s, c :: bit) = ADDER_Hex a b 1 \<longrightarrow>
-  (Hex_to_nat a) + (Hex_to_nat b) + 1 = (if (c=1) then 16 else 0) + (Hex_to_nat s)"
-  using ADDER_Hex_check_carry2 ADDER_Hex_check_carry3 by auto
+corollary ADDER_Hex_small: "(Hex_to_nat a) + (Hex_to_nat b) < 16 \<longrightarrow> (s,0 :: bit) = ADDER_Hex a b 0 \<longrightarrow> (Hex_to_nat a) + (Hex_to_nat b) = (Hex_to_nat s)"
+  using ADDER_Hex_check2 by blast
 
 theorem ADDER_Hex_comm: "ADDER_Hex a b c = ADDER_Hex b a c"
-proof (cases a)
-  case A: (Hex a1 a2 a3 a4)
-  then show ?thesis
-  proof (cases b)
-    case (Hex b1 b2 b3 b4)
-    then show ?thesis by (simp add: A FULLADDER_comm)
-  qed
-qed
+  by (case_tac a; case_tac b) (simp add: FULLADDER_comm)
 
 (* Add two words together, does not signal overflow or underflow, discards carry bit. *)
 fun ADDER16 :: \<open>Word \<Rightarrow> Word \<Rightarrow> Word\<close> where
-"ADDER16 (Word a1 a2 a3 a4) (Word b1 b2 b3 b4) = (let (s4,c4) = ADDER_Hex a4 b4 0
-in let (s3,c3) = ADDER_Hex a3 b3 c4
-in let (s2,c2) = ADDER_Hex a2 b2 c3
-in let (s1,c1) = ADDER_Hex a1 b1 c2
-in (Word s1 s2 s3 s4))"
+  "ADDER16 (Word a1 a2 a3 a4) (Word b1 b2 b3 b4) = (let (s4,c4) = ADDER_Hex a4 b4 0
+  in let (s3,c3) = ADDER_Hex a3 b3 c4
+  in let (s2,c2) = ADDER_Hex a2 b2 c3
+  in let (s1,c1) = ADDER_Hex a1 b1 c2
+  in (Word s1 s2 s3 s4))"
 
 lemma ADDER16_alias: "(s4,c4) = ADDER_Hex a4 b4 0 \<and> (s3,c3) = ADDER_Hex a3 b3 c4
   \<and> (s2,c2) = ADDER_Hex a2 b2 c3 \<and> (s1,c1) = ADDER_Hex a1 b1 c2
  \<longrightarrow> ADDER16 (Word a1 a2 a3 a4) (Word b1 b2 b3 b4) = (Word s1 s2 s3 s4)"
   by (metis (no_types, lifting) ADDER16.simps split_conv)
 
-lemma ADDER16_alias2: "(s4,c4) = ADDER_Hex a4 b4 0 \<longrightarrow> (s3,c3) = ADDER_Hex a3 b3 c4
-  \<longrightarrow> (s2,c2) = ADDER_Hex a2 b2 c3 \<longrightarrow> (s1,c1) = ADDER_Hex a1 b1 c2
- \<longrightarrow> ADDER16 (Word a1 a2 a3 a4) (Word b1 b2 b3 b4) = (Word s1 s2 s3 s4)"
-  by (metis (no_types, lifting) ADDER16.simps split_conv)
-
 lemma ADDER16_0b: "ADDER16 (Word 0 0 0 0) b = b"
-proof (cases b)
-  case B: (Word b1 b2 b3 b4)
-  then show ?thesis by (simp add: ADDER_Hex_0b0 zero_Hex_def)
-qed
+  by (case_tac b) (simp add: ADDER_Hex_0b0 zero_Hex_def)
 
 lemma ADDER16_a0: "ADDER16 a (Word 0 0 0 0) = a"
-proof (cases a)
-  case (Word a1 a2 a3 a4)
-  then show ?thesis by (simp add: ADDER_Hex_a00 zero_Hex_def)
-qed
+  by (case_tac a) (simp add: ADDER_Hex_a00 zero_Hex_def)
 
 lemma ADDER16_check: "Word_to_nat (ADDER16 a b) = ((Word_to_nat a) + (Word_to_nat b)) mod 65536"
 proof (cases a)
@@ -804,32 +734,7 @@ proof (cases a)
 qed
 
 theorem ADDER16_comm: "ADDER16 x y = ADDER16 y x"
-proof (cases x)
-  case A1: (Word x1 x2 x3 x4)
-  then show ?thesis
-  proof (cases y)
-    case (Word y1 y2 y3 y4)
-    then show ?thesis by (simp add: A1 ADDER_Hex_comm)
-  qed
-qed
-
-lemma FULLADDER_assoc_fst: "(sxy,cxy) = FULLADDER x y c1 \<and> (syz,cyz) = FULLADDER y z c2
-\<longrightarrow> fst (FULLADDER sxy z c2) = fst (FULLADDER x syz c1)"
-proof (cases x)
-  case A1: zero
-  then have "FULLADDER sxy z c2 \<noteq> FULLADDER x syz c1 \<or> fst (FULLADDER sxy z c2) = fst (FULLADDER x syz c1)"
-      by auto
-  then show ?thesis
-    by (smt (z3) A1 FULLADDER_00c FULLADDER_011 FULLADDER_0b0 FULLADDER_110 FULLADDER_111 FULLADDER_comm bit_not_one_iff fst_conv)
-next
-  case one
-  then show ?thesis
-    by (smt (z3) FULLADDER_000 FULLADDER_001 FULLADDER_010 FULLADDER_011 FULLADDER_100 FULLADDER_101 FULLADDER_110 FULLADDER_111 bit_not_zero_iff fst_conv)
-qed
-
-lemma FULLADDER_assoc_snd: "(sxy,cxy) = FULLADDER x y c1 \<and> (syz,cyz) = FULLADDER y z c2
-\<longrightarrow> XOR cxy (snd (FULLADDER sxy z c2)) = XOR cyz (snd (FULLADDER x syz c1))"
-  by (smt (z3) FULLADDER_000 FULLADDER_001 FULLADDER_010 FULLADDER_011 FULLADDER_100 FULLADDER_101 FULLADDER_110 FULLADDER_111 Pair_inject XOR_0_1 XOR_1_0 bit_not_one_iff eq_snd_iff)
+  by (case_tac x; case_tac y) (simp add: ADDER_Hex_comm)
 
 theorem Word_to_nat_to_Word: "nat_to_Word (Word_to_nat a) = a"
 proof (cases a)
@@ -917,33 +822,17 @@ proof-
   then show ?thesis using Word_to_nat_injective by simp
 qed
 
-fun ADDER4 :: \<open>Hex \<Rightarrow> Hex \<Rightarrow> Hex\<close> where
-"ADDER4 a b = fst (ADDER_Hex a b 0)"
+lemma FULLADDER_x_not_x: "FULLADDER x (NOT x) 0 = (1, 0)"
+  by (metis FULLADDER_010 FULLADDER_100 NOT_0 NOT_1 bit.exhaust)
 
-fun INC4 :: \<open>Hex \<Rightarrow> Hex\<close> where
-"INC4 h = ADDER4 h 1"
+lemma ADDER_Hex_x_not_x_0: "ADDER_Hex x (NOT_Hex x) 0 = (XF,0)"
+   using FULLADDER_x_not_x by (case_tac x) force
 
-lemma ADDER4_a0: "ADDER4 a 0 = a"
-proof-
-  have "ADDER_Hex a 0 0 = (a,0)" by (simp add: ADDER_Hex_a00 zero_Hex_def)
-  moreover have "fst (ADDER_Hex a 0 0) = fst (a,0)" by (simp add: calculation)
-  ultimately have "ADDER4 a 0 = a" by simp
-  then show ?thesis by simp
-qed
-
-lemma ADDER4_comm: "ADDER4 a b = ADDER4 b a" by (simp add: ADDER_Hex_comm)
+lemma ADDER16_x_not_x: "ADDER16 x (NOT16 x) = (Word XF XF XF XF)"
+  using ADDER_Hex_x_not_x_0 ADDER16_alias by (case_tac x) auto
 
 fun INC16 :: \<open>Word \<Rightarrow> Word\<close> where
-"INC16 a = ADDER16 a (Word 0 0 0 1)"
-
-lemma INC4_f: "INC4 (Hex 1 1 1 1) = 0"
-proof-
-  have "FULLADDER 1 1 0 = (0,1) \<and> FULLADDER 1 0 1 = (0,1) \<and> FULLADDER 1 0 1 = (0,1) \<and> FULLADDER 1 0 1 = (0,1)" by simp
-  then have "ADDER_Hex (Hex 1 1 1 1) 1 0 = (Hex 0 0 0 0,1)"
-    by (simp add: one_Hex_def)
-  then show ?thesis
-    by (simp add: zero_Hex_def)
-qed
+  "INC16 a = ADDER16 a (Word 0 0 0 1)"
 
 lemma INC16_fffe: "INC16 (Word XF XF XF XE) = (Word XF XF XF XF)"
   by (simp add: ADDER16_a0 one_Hex_def zero_Hex_def)
@@ -951,10 +840,19 @@ lemma INC16_fffe: "INC16 (Word XF XF XF XE) = (Word XF XF XF XF)"
 lemma INC16_ffff: "INC16 (Word XF XF XF XF) = (Word 0 0 0 0)"
   by (simp add: one_Hex_def zero_Hex_def)
 
+lemma "INC16 (ADDER16 x (NOT16 x)) = Word 0 0 0 0"
+  using ADDER16_x_not_x INC16_ffff by auto
+
+lemma INC_swaps_ADD16: "y = (Word XF XF XF XF) \<longrightarrow> ADDER16 x (INC16 y) = INC16 (ADDER16 x y)"
+  using ADDER16_assoc INC16.simps by presburger
+
 section \<open>Arithmetic Logical Unit\<close>
 
 fun NEGATE16 :: \<open>Word \<Rightarrow> Word\<close> where
-"NEGATE16 w = INC16 (NOT16 w)"
+  "NEGATE16 w = INC16 (NOT16 w)"
+
+lemma NEGATE_swap_inc: "ADDER16 (Word 0 0 0 1) (NOT16 x) = NEGATE16 x"
+  by (simp add: ADDER16_comm)
 
 lemma NEGATE16_zero: "NEGATE16 (Word 0 0 0 0) = (Word 0 0 0 0)"
   by (metis (mono_tags, lifting) INC16_ffff NEGATE16.elims NOT16.simps NOT_0 NOT_Hex.simps zero_Hex_def)
@@ -966,91 +864,55 @@ lemma INC_negate_one: "INC16 (NEGATE16 (Word 0 0 0 1)) = Word 0 0 0 0"
   using INC16_ffff NEGATE16_one by presburger
 
 fun SUB16 :: \<open>Word \<Rightarrow> Word \<Rightarrow> Word\<close> where
-"SUB16 x y = ADDER16 x (NEGATE16 y)"
-
-lemma FULLADDER_x_not_x: "FULLADDER x (NOT x) 0 = (1, 0)"
-  by (metis FULLADDER_010 FULLADDER_100 NOT_0 NOT_1 bit.exhaust)
-
-lemma ADDER_Hex_x_not_x_0: "ADDER_Hex x (NOT_Hex x) 0 = (XF,0)"
-proof (cases x)
-  case (Hex x1 x2 x3 x4)
-  then show ?thesis using FULLADDER_x_not_x by force
-qed
-
-lemma ADDER16_x_not_x: "ADDER16 x (NOT16 x) = (Word XF XF XF XF)"
-proof (cases x)
-  case A1: (Word x1 x2 x3 x4)
-  have A2: "(XF,0) = ADDER_Hex x4 (NOT_Hex x4) 0
-\<and> (XF,0) = ADDER_Hex x3 (NOT_Hex x3) 0
-\<and> (XF,0) = ADDER_Hex x2 (NOT_Hex x2) 0
-\<and> (XF,0) = ADDER_Hex x1 (NOT_Hex x1) 0" by (simp add: ADDER_Hex_x_not_x_0)
-  have "x = (Word x1 x2 x3 x4)
-\<and> NOT16 x = (Word (NOT_Hex x1) (NOT_Hex x2) (NOT_Hex x3) (NOT_Hex x4))"
-    using A1 by simp
-  then show ?thesis
-    using A2 ADDER16_alias by auto
-qed
-
-lemma "INC16 (ADDER16 x (NOT16 x)) = Word 0 0 0 0"
-  using ADDER16_x_not_x INC16_ffff by auto
-
-lemma INC_swaps_ADD16: "y = (Word XF XF XF XF) \<longrightarrow> ADDER16 x (INC16 y) = INC16 (ADDER16 x y)"
-  using ADDER16_assoc INC16.simps by presburger
-
-lemma NEGATE_swap_inc: "ADDER16 (Word 0 0 0 1) (NOT16 x) = NEGATE16 x"
-  by (simp add: ADDER16_comm)
+  "SUB16 x y = ADDER16 x (NEGATE16 y)"
 
 lemma SUB16_x_x: "SUB16 x x = (Word 0 0 0 0)"
   using ADDER16_assoc ADDER16_x_not_x INC_negate_one NEGATE16_one by auto
 
 fun DEC16 :: \<open>Word \<Rightarrow> Word\<close> where
-"DEC16 x = SUB16 x (Word 0 0 0 1)"
+  "DEC16 x = SUB16 x (Word 0 0 0 1)"
 
 lemma DEC_is_add_neg: "DEC16 x = ADDER16 x (NEGATE16 (Word 0 0 0 1))" by simp 
 
 lemma DEC_as_minus_one_plus_y: "ADDER16 (NEGATE16 (Word 0 0 0 1)) x = DEC16 x" 
   using ADDER16_comm by auto
 
-lemma NOT16_zero: "NOT16 (Word 0 0 0 0) = Word XF XF XF XF"
-  by (simp add: zero_Hex_def)
-
-
 lemma NEGATE_iff_sums_to_zero: "y = NEGATE16 x \<longleftrightarrow> ADDER16 x y = (Word 0 0 0 0)"
   by (metis (no_types) ADDER16_0b ADDER16_assoc SUB16.elims SUB16_x_x)
 
 fun ZERO_OUT_WORD :: \<open>Word \<Rightarrow> bit \<Rightarrow> Word\<close> where
-"ZERO_OUT_WORD w zr = MUX16 w (Word 0 0 0 0) zr"
+  "ZERO_OUT_WORD w zr = MUX16 w (Word 0 0 0 0) zr"
 
 lemma ZERO_OUT_WORD_isZero: "ISZERO16 (ZERO_OUT_WORD w 1) = 1"
   using ISZERO16_zero by auto
 
 fun NOT_WORD :: \<open>Word \<Rightarrow> bit \<Rightarrow> Word\<close> where
-"NOT_WORD w ng = MUX16 w (NOT16 w) ng"
+  "NOT_WORD w ng = MUX16 w (NOT16 w) ng"
 
 fun ZERO_OR_NOT :: \<open>Word \<Rightarrow> bit \<Rightarrow> bit \<Rightarrow> Word\<close> where
-"ZERO_OR_NOT w zr ng = (NOT_WORD (ZERO_OUT_WORD w zr) ng)"
+  "ZERO_OR_NOT w zr ng = (NOT_WORD (ZERO_OUT_WORD w zr) ng)"
 
-lemma ZERO_OR_NOT_w00 [simp]: "ZERO_OR_NOT w 0 0 = w" by simp
+lemma ZERO_OR_NOT_w00: "ZERO_OR_NOT w 0 0 = w" by simp
 
-lemma ZERO_OR_NOT_w01 [simp]: "ZERO_OR_NOT w 0 1 = NOT16 w" by simp
+lemma ZERO_OR_NOT_w01: "ZERO_OR_NOT w 0 1 = NOT16 w" by simp
 
-lemma ZERO_OR_NOT_w10 [simp]: "ZERO_OR_NOT w 1 0 = (Word 0 0 0 0)" by simp
+lemma ZERO_OR_NOT_w10: "ZERO_OR_NOT w 1 0 = (Word 0 0 0 0)" by simp
 
 lemma ZERO_OR_NOT_w11 [simp]: "ZERO_OR_NOT w 1 1 = (Word XF XF XF XF)"
   using NOT16_zero by auto
 
 fun ADDER16_OR_AND16 :: \<open>Word \<Rightarrow> Word \<Rightarrow> bit \<Rightarrow> Word\<close> where
-"ADDER16_OR_AND16 a b f = MUX16 (AND16 a b) (ADDER16 a b) f"
+  "ADDER16_OR_AND16 a b f = MUX16 (AND16 a b) (ADDER16 a b) f"
 
-lemma ADDER_OR_AND_ab1 [simp]: "ADDER16_OR_AND16 a b 1 = ADDER16 a b"
+lemma ADDER_OR_AND_ab1: "ADDER16_OR_AND16 a b 1 = ADDER16 a b"
   by simp
 
-lemma ADDER_OR_AND_ab0 [simp]: "ADDER16_OR_AND16 a b 0 = AND16 a b"
+lemma ADDER_OR_AND_ab0: "ADDER16_OR_AND16 a b 0 = AND16 a b"
   by simp
 
 (* The ALU operation without transforming the output. *)
 fun ALU_op :: \<open>Word \<Rightarrow> Word \<Rightarrow> bit \<Rightarrow> bit \<Rightarrow> bit \<Rightarrow> bit \<Rightarrow> bit \<Rightarrow> Word\<close> where
-"ALU_op x y zx nx zy ny f = (ADDER16_OR_AND16 (ZERO_OR_NOT x zx nx) (ZERO_OR_NOT y zy ny) f)"
+  "ALU_op x y zx nx zy ny f = (ADDER16_OR_AND16 (ZERO_OR_NOT x zx nx) (ZERO_OR_NOT y zy ny) f)"
 
 lemma ALU_11111: "ALU_op x y 1 1 1 1 1 = Word XF XF XF XE"
   using ADDER_OR_AND_ab1 ZERO_OR_NOT_w11 by auto
@@ -1062,7 +924,8 @@ lemma ALU_op_00110: "ALU_op x y 0 0 1 1 0 = x"
   using AND16_x_FFFF NOT16_zero by auto
 
 lemma ALU_op_00111: "ALU_op x y 0 0 1 1 1 = DEC16 x"
-  using ADDER_OR_AND_ab1 ALU_op.simps DEC_is_add_neg NEGATE16_one ZERO_OR_NOT_w00 ZERO_OR_NOT_w11 by presburger
+  using ADDER_OR_AND_ab1 ALU_op.simps DEC_is_add_neg NEGATE16_one ZERO_OR_NOT_w00 ZERO_OR_NOT_w11
+  by presburger
 
 lemma ALU_op_01001: "ALU_op x y 0 1 0 0 1 = ADDER16 (NOT16 x) y"
   by simp
@@ -1071,7 +934,8 @@ lemma ALU_op_01111: "ALU_op x y 0 1 1 1 1 = DEC16 (NOT16 x)"
   using INC16_fffe NOT16_one by auto
 
 lemma NOT_DEC_NOT_is_INC: "NOT16 (DEC16 (NOT16 x)) = INC16 x"
-  by (metis (no_types, opaque_lifting) ADDER16_0b ADDER16_assoc DEC16.elims DEC_as_minus_one_plus_y INC16.elims NEGATE16.elims SUB16.elims SUB16_x_x)
+  by (metis (no_types, opaque_lifting) ADDER16_0b ADDER16_assoc DEC16.elims DEC_as_minus_one_plus_y
+      INC16.elims NEGATE16.elims SUB16.elims SUB16_x_x)
 
 lemma ALU_op_11000: "ALU_op x y 1 1 0 0 0 = y"
   using AND16_FFFF_x NOT16_zero by auto
@@ -1080,13 +944,15 @@ lemma ALU_op_11001: "ALU_op x y 1 1 0 0 1 = DEC16 y"
 proof-
   have "ALU_op x y 1 1 0 0 1 = ADDER16 (NOT16 (Word 0 0 0 0)) y" by auto
   then show ?thesis
-    by (metis (no_types, lifting) ADDER16.simps ADDER16_a0 ADDER_Hex_simps DEC_as_minus_one_plus_y FULLADDER_010 FULLADDER_100 INC16.simps NEGATE16.simps NOT16.simps NOT_0 NOT_1 NOT_Hex.simps one_Hex_def zero_Hex_def)
+    by (metis (no_types, lifting) ADDER16.simps ADDER16_a0 ADDER_Hex_simps DEC_as_minus_one_plus_y
+        FULLADDER_010 FULLADDER_100 INC16.simps NEGATE16.simps NOT16.simps NOT_0 NOT_1 NOT_Hex.simps
+        one_Hex_def zero_Hex_def)
 qed
 
 fun ALU :: \<open>Word \<Rightarrow> Word \<Rightarrow> bit \<Rightarrow> bit \<Rightarrow> bit \<Rightarrow> bit \<Rightarrow> bit \<Rightarrow> bit \<Rightarrow> Word * bit * bit\<close> where
-"ALU x y zx nx zy ny f no = (let sym = ALU_op x y zx nx zy ny f
-in let output = MUX16 sym (NOT16 sym) no
-in (output, ISZERO16 output, sign_bit output))"
+  "ALU x y zx nx zy ny f no = (let sym = ALU_op x y zx nx zy ny f
+  in let output = MUX16 sym (NOT16 sym) no
+  in (output, ISZERO16 output, sign_bit output))"
 
 text \<open>To prove correctness of the ALU implementation, we should check each of the 19 cases for the
 possible outputs.\<close>
@@ -1141,7 +1007,6 @@ theorem ALU_110010: "ALU x y 1 1 0 0 1 0 = (DEC16 y, ISZERO16 (DEC16 y), sign_bi
 theorem ALU_000010: "ALU x y 0 0 0 0 1 0 = (ADDER16 x y, ISZERO16 (ADDER16 x y), sign_bit (ADDER16 x y))"
   by (smt (z3) ADDER_OR_AND_ab1 ALU.simps ALU_op.simps MUX16_left NOT_WORD.simps 
       ZERO_OR_NOT.simps ZERO_OUT_WORD.simps)
-(* by (metis ADDER_OR_AND_ab1 ALU.simps ALU_op.simps MUX16_left NEGATE_WORD.simps ZERO_OR_NEGATE.simps ZERO_OUT_WORD.simps) *)
 
 lemma ADD_NOT_x_y: "NOT16 (ADDER16 (NOT16 x) y) = SUB16 x y"
 proof -
@@ -1162,7 +1027,14 @@ theorem ALU_000000: "ALU x y 0 0 0 0 0 0 = (AND16 x y, ISZERO16 (AND16 x y), sig
       ZERO_OR_NOT.simps ZERO_OUT_WORD.simps)
 
 theorem ALU_010101: "ALU x y 0 1 0 1 0 1 = (OR16 x y, ISZERO16 (OR16 x y), sign_bit (OR16 x y))"
-  by (smt (verit) ADDER16_OR_AND16.simps ALU.simps ALU_op.simps MUX16_left NOT_WORD.simps
-      NOT16_AND16_NOT16 ZERO_OR_NOT.simps ZERO_OR_NOT_w01 ZERO_OUT_WORD.simps)
+proof - (* 81 ms *)
+  have "\<forall>b w ba. ZERO_OR_NOT w ba b = NOT_WORD (MUX16 w (Word 0 0 0 0) ba) b"
+    using ZERO_OR_NOT.simps ZERO_OUT_WORD.simps by presburger
+  moreover have "\<forall>w. NOT16 w = NOT_WORD (MUX16 w (Word 0 0 0 0) 0) 1"
+    by simp
+  ultimately show ?thesis
+    by (smt (z3) ADDER16_OR_AND16.simps ALU.simps ALU_op.simps MUX16_left NOT16_AND16_NOT16
+        NOT_WORD.simps)
+qed
 
 end
